WIP; fixing Cellio example

examples/cellio/CellioIAproof.v
@@ -1,6 +1,7 @@
 Require Import CRIS.
 Require Import CellioHeader CellioA CellioI.
 Require Import InputA.
+Require Import wsim_tactics.
 
 Set Implicit Arguments.
 
@@ -10,68 +11,78 @@ Module CellioIA. Section CellioIA.
   Import CellioA.
   Context `{!invG α Σ Γ, !subG Γ Σ, !sinvG Σ Γ α β τ, !CellioAGΓ Γ}.
 
-  Variable ginv: invspec.
-  Variable SpcG: string -> option fspec.
-  Hypothesis InputInSpcG: spc_incl InputAS.Spc SpcG.
-
-  Definition Ist: nat -> alist key Any.t -> alist key Any.t -> iProp Σ :=
+  (* 1) universe ids of src/tgt modules *)
+  Context (u_a u_i : univ_id).
+  (* 2) stratification level *)
+  Context (n : level).
+  (* 3) global invariant for src module *)
+  Context (ginv : invspec).
+  (* 4) spc for src module *)
+  Context (Spc_s : string → option fspec).
+  Context (InputInSpcG : spc_incl InputAS.Spc Spc_s).
+  
+  Definition Ist : nat → alist key Any.t → alist key Any.t → iProp Σ :=
     λ _ st_src st_tgt,
       (∃ v, ⌜st_tgt = [(CellioI.v_cv, v↑)]⌝ ∗ auth v)%I.
 
   Local Notation CellioI := (CellioI.t).
-  Local Notation CellioA := (CellioA.t ginv SpcG).
+  Local Notation CellioA := (CellioA.t ginv Spc_s).
 
   Lemma simF_set : HSim.sim_fun open CellioA CellioI Ist CellioName.set.
   Proof.
-    init_simF.
+    init_wsim u_a u_i n.
 
-    steps_l. iDestruct "ASM" as "%"; subst.
+    w_steps_l. iDestruct "ASM" as "->".
+    w_force_l tt. w_forces_l. iSplit; first eauto.
 
-    force_l tt. forces_l. iSplitL ""; eauto.
-    call "IST"; eauto.
-    steps_l. iDestruct "ASM" as "%"; subst.
+    w_call "IST"; eauto.
+    w_steps_l. iDestruct "ASM" as "->".
 
     iDestruct "IST" as (v) "(% & AUTH)". subst.
 
     iPoseProof (cell_auth_get with "ASM' AUTH") as "%"; subst.
     iMod (cell_auth_set with "ASM' AUTH") as "(C & A)".
 
-    forces_l. iSplitL "C"; eauto.
+    w_forces_l. iSplitL "C"; eauto.
 
-    steps_r. hss. steps_r. steps_l. forces_l.
-    iSplitL ""; eauto.
+    w_steps_r. hss. w_steps_r. w_steps_l. w_forces_l.
+    iSplit; eauto.
 
-    step.
+    w_step.
     iSplitL ""; eauto.
     iExists _. iFrame. eauto.
   Qed.
   
-  Lemma simF_get:
-    HSim.sim_fun open CellioA CellioI Ist CellioName.get.
+  Lemma simF_get : HSim.sim_fun open CellioA CellioI Ist CellioName.get.
   Proof.
-    init_simF.
+    init_wsim u_a u_i n.
 
-    steps_l. iDestruct "ASM" as "%"; subst.
+    w_steps_l. iDestruct "ASM" as "->".
     iDestruct "IST" as (v) "(% & AUTH)". subst.
 
     iPoseProof (cell_auth_get with "ASM' AUTH") as "%"; subst.
 
-    steps_r. hss. steps_r. forces_l.
-    iSplitL "ASM'"; eauto.
+    w_steps_r. hss. w_steps_r.
+    w_forces_l. iSplitL "ASM'"; eauto.
     
-    steps_l. forces_l.
-    iSplitL ""; eauto.
+    w_steps_l. w_forces_l. iSplit; eauto.
 
-    step.
-    iSplitL ""; eauto.
+    w_step. iSplit; eauto.
     iExists _. iFrame. eauto.
   Qed.
   
-  Theorem sim: HSim.t open CellioA CellioI CellioA.InitCond Ist.
+  Lemma sim : HSim.t open CellioA CellioI CellioA.InitCond Ist.
   Proof.
     init_sim.
     - iIntros "H". iExists _. iFrame. eauto.
     - apply simF_set; eauto.
     - apply simF_get; eauto.
   Qed.
+  End CellioIA.
+
+  Section CellioIA.
+    Context `{!invG α Σ Γ, !subG Γ Σ, !sinvG Σ Γ α β τ, !CellioAGΓ Γ}.
+    Lemma wctxr (n : level) ginv Spc_s (InputInSpc : spc_incl InputAS.Spc Spc_s) :
+      w_ctx_refines (λ _, CellioA.t ginv Spc_s, CellioA.InitCond) (λ _, CellioI.t, emp%I).
+    Proof. exists 1%positive; intros u v Huv; s; eapply main_adequacy, sim; ss. Qed.
 End CellioIA. End CellioIA.
